added local tactics for Cheriot

Cheriot/CoreConfig.v
@@ -1,5 +1,7 @@
 Require Import Kami.AllNotations.
+
 Require Import ProcKami.Cheriot.Lib ProcKami.Cheriot.Types ProcKami.Cheriot.InstSpec ProcKami.Cheriot.RunSpec.
+Require Import ProcKami.Cheriot.Tactics.
 
 Section Prefix.
   Context `{coreConfigParams: CoreConfigParams}.
@@ -11,7 +13,7 @@ Section Prefix.
   Definition specRules : list RuleT :=
     (@^"specTimerIncAndInterruptSetRule", specTimerIncAndInterruptSetRule) ::
       (@^"specTimerInterruptTakeRule", specTimerInterruptTakeRule scrList csrList) ::
-      (@^"specInstBoundsExpcetionRule", specInstBoundsExceptionRule scrList csrList) ::
+      (@^"specInstBoundsExceptionRule", specInstBoundsExceptionRule scrList csrList) ::
       (@^"specInstIllegalExceptionRule", fun ty => specInstIllegalExceptionRule scrList csrList ty specInstEntries) ::
       map (fun ie => (@^(append "specDecExecRule_" (instName ie)), fun ty => specDecExecRule scrList csrList ty ie))
       specInstEntries.
@@ -56,67 +58,70 @@ Section Prefix.
 
   Definition specBaseMod: BaseModule := BaseMod specRegs specRules [].
 
-  Ltac conjunctionRepeatConstructors :=
-    match goal with
-    | |- ?A /\ ?B => constructor; conjunctionRepeatConstructors
-    | |- _ => idtac
-    end.
-
-  Local Ltac constructor_simpl :=
-    econstructor; eauto; simpl; unfold not; intros.
-
-  Ltac murali := match goal with
-                 | |- @WfBaseModule_new _ _ => unfold WfBaseModule_new
-                 | |- @WfMod_new _ _ => constructor_simpl
-                 | |- _ /\ _ => constructor_simpl
-                 | |- @WfActionT_new _ _ _ (convertLetExprSyntax_ActionT ?e) => apply WfLetExprSyntax_new
-                 | |- @WfActionT_new _ _ _ _ => constructor_simpl
-                 | |- NoDup _ => constructor_simpl
-                 | H: _ \/ _ |- _ => destruct H; subst; simpl
-                 | |- forall _, _ => intros
-                 | |- _ -> _ => intros 
-                 | H: In _ (getAllMethods _) |- _ => simpl in H;inversion H;subst;clear H;simpl
-                 | |- _ => unfold lookup; simpl; repeat rewrite strip_pref
-                 end; unfold lookup; simpl; repeat rewrite strip_pref; simpl.
-
-  (*
-  Theorem WfSpecDecRule: forall ie ty, WfActionT_new specRegs (specDecExecRule scrList csrList ty ie).
+  Theorem WfSpecDecExecRule: forall ie ty, WfActionT specRegs (specDecExecRule scrList csrList ty ie).
   Proof.
     cbv [specRegs specDecExecRule handleException]; intros.
-    murali.
-    unfold lookup; simpl; repeat rewrite strip_pref; simpl.
-    - 
-    cbv [lookup find fst snd].
-    rewrite ?strip_pref.
-    match goal with
-    | |- context [String.eqb ?P ?Q] => cbv [P Q String.eqb Ascii.eqb Bool.eqb]
-    end.
-    discharge_wf_new.
-    - murali.
-    - 
-    test.
+    destruct hasTrap; repeat dischargeWfActionT.
   Qed.
 
-    discharge_wf_new.
-  Theorem WfSpecBaseMod: WfBaseModule_new type specBaseMod.
+  Theorem WfSpecTimerIncAndInterruptSetRule: forall ty, WfActionT specRegs (specTimerIncAndInterruptSetRule ty).
   Proof.
-    cbv [WfBaseModule_new getRegisters getRules getMethods specBaseMod specRules specRegs
-           specTimerIncAndInterruptSetRule
-           specTimerInterruptTakeRule specInstBoundsExceptionRule specInstIllegalExceptionRule specDecExecRule].
-    conjunctionRepeatConstructors.
-    - cbn [WfRules snd]; conjunctionRepeatConstructors.
-      + destruct hasTrap; discharge_wf_new.
-      + cbv [handleException]; destruct hasTrap.
-        * discharge_wf_new.
-      + 
-      + 
+    cbv [specRegs specTimerIncAndInterruptSetRule handleException]; intros.
+    destruct hasTrap; repeat dischargeWfActionT.
+  Qed.
+
+  Theorem WfSpecTimerInterruptTakeRule: forall ty, WfActionT specRegs (specTimerInterruptTakeRule scrList csrList ty).
+  Proof.
+    cbv [specRegs specTimerInterruptTakeRule handleException]; intros.
+    destruct hasTrap; repeat dischargeWfActionT.
+  Qed.
+
+  Theorem WfSpecInstBoundsExceptionRule:
+    forall ty, WfActionT specRegs (specInstBoundsExceptionRule scrList csrList ty).
+  Proof.
+    cbv [specRegs specInstBoundsExceptionRule handleException]; intros.
+    destruct hasTrap; repeat dischargeWfActionT.
+  Qed.
+
+  Theorem WfSpecInstIllegalExceptionRule:
+    forall ty, WfActionT specRegs (specInstIllegalExceptionRule scrList csrList ty specInstEntries).
+  Proof.
+    cbv [specRegs specInstIllegalExceptionRule handleException]; intros.
+    destruct hasTrap; repeat dischargeWfActionT.
+  Qed.
+
+  Ltac instEntriesNoDup :=
+    cbv [specInstEntries]; destruct hasTrap; cbn [map fst instName mkLdInst mkStInst mkBranchInst mkCsrEntry append];
+    commonPrefixNoDup.
+
+  Theorem NoDupSpecRules: NoDup (map fst specRules).
+  Proof.
+    cbn [specRules map fst].
+    rewrite map_map.
+    instEntriesNoDup.
+  Qed.
+  
+  Theorem WfSpecBaseMod: WfBaseModule type specBaseMod.
+  Proof.
+    cbv [WfBaseModule getRegisters getRules getMethods specBaseMod].
+    repeatConj.
+    - cbv [specRules]; cbn [In]; let rule := fresh "rule" in intro rule; rewrite in_map_iff; intros.
+      repeat match goal with
+             | H: _ \/ _ |- _ => destruct H
+             | H: _ /\ _ |- _ => destruct H
+             | H: exists x, _ |- _ => destruct H
+             | H: _ = rule |- _ => rewrite <- H; clear H rule;
+                                   cbn [snd]
+             end.
+      + apply WfSpecTimerIncAndInterruptSetRule.
+      + apply WfSpecTimerInterruptTakeRule.
+      + apply WfSpecInstBoundsExceptionRule.
+      + apply WfSpecInstIllegalExceptionRule.
+      + apply WfSpecDecExecRule.
+    - cbv [In].
+      intros; tauto.
     - constructor.
-    - constructor.
-    - destruct hasTrap; cbv [map fst];
-        apply (NoDup_map_inv (rmStringPrefix (String.length (procName ++ "_"))%string)); cbv [map];
-        rewrite ?rmAppend; discharge_wf_new.
-    - destruct hasTrap; cbv [map fst specInstEntries instName mkLdInst mkStInst mkBranchInst mkCsrEntry];
-        cbn [append]; discharge_wf_new.
-  Admitted.
-*)
+    - cbv [specRegs]; instEntriesNoDup.
+    - apply NoDupSpecRules.
+  Qed.
 End Prefix.
