Cheriot/Tactics.v
@@ -1,0 +1,40 @@
+Require Import Kami.AllNotations ProcKami.Cheriot.Lib ProcKami.Cheriot.Types ProcKami.Cheriot.InstSpec.
+
+Ltac getOrIntrosLtacHelp val ls :=
+  match ls with
+  | (val, _) :: _ => uconstr:(or_introl eq_refl)
+  | (?x, _) :: ?xs => let y := getOrIntrosLtacHelp val xs in uconstr:(or_intror y)
+  end.
+
+Ltac dischargeWfActionT :=
+  cbv [regName scrRegInfo csrRegInfo filter];
+  match goal with
+  | |- @WfActionT _ _ _ (convertLetExprSyntax_ActionT ?e) => apply WfLetExprSyntax_regs
+  | |- @WfActionT _ _ _ _ => econstructor; eauto
+  | |- In (?val, _) (getKindAttr ?ls) =>
+      let y := (getOrIntrosLtacHelp val ls) in exact y
+  | |- forall _, _ => intros
+  | |- _ -> _ => intros 
+  end.
+
+Ltac getOrIntrosLtac :=
+  match goal with
+  | |- In (?val, _) (getKindAttr ?ls) =>
+      let y := (getOrIntrosLtacHelp val ls) in exact y
+  end.
+
+Ltac repeatConj :=
+  repeat match goal with
+    | |- ?A /\ ?B => apply conj
+    | |- _ => idtac
+    end.
+
+Ltac simpleNoDup :=
+  match goal with
+  | |- NoDup _ => apply (NoDupEvalCorrect1 String.eqb String.eqb_eq); auto
+  end.
+
+Ltac commonPrefixNoDup :=
+  apply (NoDup_map_inv (rmStringPrefix (String.length (procName ++ "_"))%string)); cbv [map];
+  rewrite ?rmAppend; simpleNoDup.
+
